@prefix ifn3: <https://datos.iepnb.es/def/sector-publico/medio-ambiente/ifn3/> .
@prefix kTaxon: <https://datos.iepnb.es/kos/sector-publico/medio-ambiente/ifnTop/taxon/> .
@prefix owl: <http://www.w3.org/2002/07/owl#> .
@prefix rdfs: <http://www.w3.org/2000/01/rdf-schema#> .
@prefix rdf: <http://www.w3.org/1999/02/22-rdf-syntax-ns#> .
# @prefix xml: <http://www.w3.org/XML/1998/namespace> .


ifn3:PlantSpecies rdf:type owl:Class ;
    rdfs:subClassOf kTaxon:KingdomPlantae ;
    rdfs:label "Especie vegetal"@en , "Plant Species"@en ;
    rdfs:comment "Especie vegetal, tal y como se ha registrado en el inventario. Es posible que los individuos de esta clase no sean estrictamente especies Genus, sub-genus, y mezclas de especies son también individuos posibles."@es , "Plant species, as recorded in the inventory. It is possible that the individuals of this class are not strictly species, but genus, sub-genus, mix of species, etc."@en ;rdfs:label "Especie vegetal"@es , "Plant Species"@en ;
    rdfs:isDefinedBy ifn3: .

ifn3:TreeSpecies rdf:type owl:Class ;
    rdfs:subClassOf ifn3:PlantSpecies ;
    rdfs:label "Especie arbórea"@en , "Tree Species"@en ;
    rdfs:comment "Especie arbórea, tal y como se ha registrado en el inventario. Es posible que los individuos de esta clase no sean estrictamente especies. Genus, sub-genus, y mezclas de especies son también individuos posibles."@es , "Tree species, as recorded in the inventory. It is possible that the individuals of this class are not strictly species, but genus, sub-genus, mix of species, etc."@en ;
    rdfs:isDefinedBy ifn3: .

ifn3:BushSpecies rdf:type owl:Class ;
    rdfs:subClassOf ifn3:PlantSpecies ;
    rdfs:label "Bush Species"@en , "Especie arbustiva"@es ;
    rdfs:comment "Bush species, as recorded in the inventory. It is possible that the individuals of this class are not strictly species, but genus, sub-genus, mix of species, etc."@en , "Especie arbustiva, tal y como se ha registrado en el inventario. Es posible que los individuos de esta clase no sean estrictamente especies. Genus, sub-genus, y mezclas de especies son también individuos posibles."@es ;
    rdfs:isDefinedBy ifn3: .

ifn3:hasScientificName rdf:type owl:ObjectProperty ;
    rdfs:label "scientific name"@en ;
    rdfs:domain ifn3:PlantSpecies ;
    rdfs:range ifn3:ScientificName ;
    rdfs:isDefinedBy ifn3: ;
.